rupicola/io/Compilation.fst
@@ -12,6 +12,7 @@ let rec compile #g #a (#s:fs_oval g a) (qs:g ⊢ s) : Tot exp (decreases qs) =
   | Qtt -> EUnit
   | QVar0 -> EVar 0
   | QVarS #g qx -> subst sub_inc (compile qx)
+  | QFd fd -> EFileDescr fd
   | QAppGhost -> EUnit
   | QApp qf qx -> EApp (compile qf) (compile qx)
   | QLambda qbody -> ELam (compile qbody)
@@ -27,8 +28,10 @@ let rec compile #g #a (#s:fs_oval g a) (qs:g ⊢ s) : Tot exp (decreases qs) =
   | QLambdaProd qbody -> ELam (compile_oprod qbody)
 and compile_oprod #g #a (#s:fs_oprod g a) (qs:oprod_quotation g s) : Tot exp (decreases qs) =
   match qs with
-  | QRead -> ERead
-  | QWrite qarg -> EWrite (compile qarg)
+  | QOpenfile qfnm -> EOpen (compile qfnm)
+  | QRead qfd -> ERead (compile qfd)
+  | QWrite qfd qmsg -> EWrite (compile qfd) (compile qmsg)
+  | QClose qfd -> EClose (compile qfd)
   | QReturn qx -> compile qx
   | QBindProd qm qk -> EApp (ELam (compile_oprod qk)) (compile_oprod qm)
   | QAppProd qf qx -> EApp (compile qf) (compile qx)
@@ -49,6 +52,7 @@ let rec compile_equiv #g (#a:qType) (#s:fs_oval g a) (qs:g ⊢ s)
   | QVarS #g' #_ #b #x qx ->
     compile_equiv qx;
     equiv_varS #g' #a #b x (compile qx)
+  | QFd fd -> equiv_file_descr g fd
   | QAppGhost -> equiv_unit g
   | QApp #_ #qa #qb #f #x qf qx ->
     compile_equiv qf;
@@ -92,10 +96,19 @@ and compile_equiv_prod #g (#a:qType) (#s:fs_oprod g a) (qs:oprod_quotation g s)
   : Lemma (ensures (s `equiv_oprod a` (compile_oprod qs))) (decreases qs)
   =
   match qs with
-  | QRead -> equiv_oprod_read g
-  | QWrite #_ #arg qarg ->
-    compile_equiv qarg;
-    equiv_oprod_write arg (compile qarg)
+  | QOpenfile #_ #fnm qfnm ->
+    compile_equiv qfnm;
+    equiv_oprod_openfile fnm (compile qfnm)
+  | QRead #_ #fd qfd ->
+    compile_equiv qfd;
+    equiv_oprod_read fd (compile qfd)
+  | QWrite #_ #fd #msg qfd qmsg ->
+    compile_equiv qfd;
+    compile_equiv qmsg;
+    equiv_oprod_write fd msg (compile qfd) (compile qmsg)
+  | QClose #_ #fd qfd ->
+    compile_equiv qfd;
+    equiv_oprod_close fd (compile qfd)
   | QReturn #_ #_ #x qx ->
     compile_equiv qx;
     equiv_oprod_return x (compile qx)
